Part 1:

 Show that the square root of 2 is irrational.
 
 sqrt(2)
 
 sqrt(2) = a/b

2= a^2/ b^2

a^2 = 2 * b^2
 
 2 = (2k)^2/b^2

2 = 4k^2/b^2

2b^2 = 4k^2

b^2 = 2k^2
 
 b^2 becomes even it is false.
 
 If n = 25, 100,169,then or  n is a perfect square and is the sum of two perfect squares.
 
 m = √n where m is an integer
 
 m = √25, √100, or √169
 
 m = 5, 10, or 13

m² = 25, 100, or 169
 
 m² = n
 
 n is a perfect square by the definition of perfect squares.
 
 n = (9 + 16), (81 + 9), or (144 + 25),
 
 9 = 3², 16 = 4², 81 = 9², 144 = 12², and 25 = 5²

n is the sum of of two perfect squares.
 
 The sum of two odd integers is even. Hint: By definition, even integers can be expressed as 2n, thus odd integers can be expressed as 

2n + 1
 
 n1 = 2k1 +1
 
 n2 = 2k2 +1
 
 (2k1 +1)+(2k2 +1)
 
 2k1 + 2k2 +2
 
 2(k1+k2+1)

because the some of the 3 integers is an integer

2k
 
 meaning the sum of two odd integers is an even integer
 

The sum of an even integer and it's square is even
 
 n = even number 
 
 n = 2m 
 
 n^2 = (2m)^2
 
 n^2 = 4m^2

then add the equation n^2 + n and have it equal this equation

n^2 + n = 4m^2 + 2m

2(2m^2 +m)
 
 2m and this equals an even number
 
 If n= odd number 
 
 n = 2m +1

n^2 = (2m+1)^2

n^2 = 4m^2 +4m +1
 
 then add the equation n^2 +n equal it to the above equation.

n^2 + n = 4m^2 + 4m +1 + 2m +1
 
 4m^2 +6m +2

2(2m^2 + 3m +1)

2m which equals an even number.
 
 If n squared is odd, then n is odd

Proving with contraposition
 
If n^2 is even, then n is even

n = 2k

n^2 = (2k)^2

4k^2

n^2 = 2(2k^2)
 
 n^2 = 2k
 
 meaning that n^2 is an even integer thus the statement is false.
 
 
 Part 2:
 
 1 + 5 + 9 + … + (4n – 3) = n(2n – 1)

Plug in 1 = 1 = 1(2 x 1 – 1) = 1

Now plug in K = l+5 + 9 +…+(4k-3) = k(2k-1)
 
 Now prove tht k + 1 is true:  

1 + 5 + 9 + … +  (4k- 3) + [4(k+ 1) – 3]

2k2 -k+4k+ 4-3

2k2 + 3k + 1

(k+ 1)( 2k + 1)
 
 (k+l)[2(k+l)-l]

k + 1 is true when k is true.
 

n^3 + 2n is divisible by 3

The base case: n = 0 0^3 +0= 0= 3*0 which is true
 
 show that (k+1) is true 
 
 (k+1)^3 + 2(k+1) = k^3 +3k +1 + 2k + 2

k^3 + 2k + 3(k^2 +k + 1)

3m + 3 (k^2 + k + 1)
 
 3(m + k^2 + k + 1)

with this proves that (k+1) is true.
 
 Prove that for n >= 1 , 9^ n-1 is divsible by 8 for all non- negative integers
 
 Proving that 9^n-1 is true so plug in 1 for n
 
 9^n -1 
 
 9^1 -1
 
 = 8 
 
 so the original function is true 
 
 then assume that the letter k is true
 
 9^n-1
 
 9^k-1
 
 9^k-1 = 8m
 
 9^k = 8m +1
 
 now with assuming that is is true you prove that k+1 is true 
 
 9^n-1
 
 9^(k+1) -1
 
 9^k * 9-1
 
 then input what 9^k equals
 
 8m+1 * 9-1
 
 8m * 9+9-1
 
 8m * 9 + 8
 
 8(9m + 1)
 
 therefore 9 ^n-1 is divisble by 8 
 
